Updated Definitions, Fixed proof of unoptimized server

demo/Server.v
@@ -11,30 +11,31 @@ Require Import Integers Intv.
 (* C-level spec : in C code:
 L1:
 int key;
-void encrypt (int input, void ( *complete)(int*))){
+void encrypt (int input, void ( *complete)(int* __ ))){
   int output = input ^ key;
   complete(&output);
 }
 
 L2:
 const int key = 42;
-void encrypt (int input, void ( *complete)(int*)){
+void encrypt (int input, void ( *complete)(int* __ )){
   int output = input ^ key;
   complete(&output)
 }
-*)
+                         *)
+                              
 Definition main_id := (42%positive).
 Definition encrypt_id := (1%positive).
 Definition key_id := (2%positive).
 Definition complete_id := (3%positive).
 
-Definition int__void_sg : signature := mksignature (AST.Tint :: nil) Tvoid cc_default.
+Definition intptr__void_sg : signature := mksignature (AST.Tlong :: nil) Tvoid cc_default.
 Definition int_fptr__void_sg : signature := mksignature (AST.Tint :: AST.Tlong :: nil) Tint cc_default.
 
 (** registers responding to above signatures*)
 
 Require Import Conventions1.
-
+(* Compute (is_callee_save Machregs.DI). *)
 (* Compute (loc_arguments int__void_sg). *)
 (* = if Archi.win64 then One (Locations.R Machregs.CX) :: nil else One (Locations.R Machregs.DI) :: nil *)
 (* Compute (loc_arguments int_fptr__void_sg). *)
@@ -55,22 +56,26 @@ Definition key_def := {|
 
 (*
 L1: 
-Pallocframe 16 8 0
+Pallocframe 24 16 0
 
 Pmov key RAX //read key from memory to RAX as argument
 Pxor RAX RDI //xor op
+Pmov RDI 8(RSP) // store the output on stack
+Plea 8(RSP) RDI // transfer the address of output as argument
 Pcall_r RSI //call function pointer
 
-Pfreeframe 16 8 0
+Pfreeframe 24 16 0
 Pret
 
 *)
 Definition code_b1: list instruction :=
-   Pallocframe 16 (Ptrofs.repr 8) Ptrofs.zero ::
+   Pallocframe 24 (Ptrofs.repr 16) Ptrofs.zero ::
      Pmovl_rm RAX (Addrmode None None (inr (key_id, Ptrofs.zero))) ::
      Pxorl_rr RDI RAX ::
-     Pcall_r RSI (int__void_sg) ::
-     Pfreeframe 16 (Ptrofs.repr 8) Ptrofs.zero ::
+     Pmov_mr_a (Addrmode (Some RSP) None (inl 8)) RDI ::
+     Pleaq RDI (Addrmode (Some RSP) None (inl 8)) ::
+     Pcall_r RSI (intptr__void_sg) ::
+     Pfreeframe 24 (Ptrofs.repr 16) Ptrofs.zero ::
      Pret ::
      nil.
 
@@ -80,7 +85,7 @@ Definition func_encrypt_b1: Asm.function :=
 Definition global_definitions_b1 : list (ident * globdef fundef unit) :=
   (key_id, Gvar key_def) ::
     (encrypt_id, Gfun(Internal func_encrypt_b1)) ::
-    (complete_id, Gfun(External (EF_external "complete" int__void_sg))) ::
+    (complete_id, Gfun(External (EF_external "complete" intptr__void_sg))) ::
   nil.
 
 Definition public_idents : list ident :=
@@ -99,6 +104,16 @@ Definition key_def_const := {|
 
 (*
 L2: 
+Pallocframe 24 16 0
+
+Pxor 42 RDI //xor op
+Pmov RDI 8(RSP) // store the output on stack
+Plea 8(RSP) RDI // transfer the address of output as argument
+Pcall_r RSI //call function pointer
+
+Pfreeframe 24 16 0
+Pret
+
 Pallocframe 16 8 0
 
 Pxori 42 RDI //read key from memory to RDI as argument
@@ -111,7 +126,9 @@ Pret
 Definition code_b2: list instruction :=
    Pallocframe 16 (Ptrofs.repr 8) Ptrofs.zero ::
      Pxorl_ri RDI (Int.repr 42) ::
-     Pcall_r RSI (int__void_sg) ::
+     Pmov_mr_a (Addrmode (Some RSP) None (inl 8)) RDI ::
+     Pleaq RDI (Addrmode (Some RSP) None (inl 8)) ::
+     Pcall_r RSI (intptr__void_sg) ::
      Pfreeframe 16 (Ptrofs.repr 8) Ptrofs.zero ::
      Pret ::
      nil.
@@ -122,7 +139,7 @@ Definition func_encrypt_b2: Asm.function :=
 Definition global_definitions_b2 : list (ident * globdef fundef unit) :=
   (key_id, Gvar key_def_const) ::
   (encrypt_id, Gfun(Internal func_encrypt_b2)) ::
-  (complete_id, Gfun(External (EF_external "complete" int__void_sg))) ::
+  (complete_id, Gfun(External (EF_external "complete" intptr__void_sg))) ::
   nil.
 
 Definition b2: program := mkprogram global_definitions_b2 public_idents main_id.
